steel/Zeta.Steel.PCMMap.fst
@@ -1,0 +1,311 @@
+module Zeta.Steel.PCMMap
+open FStar.Map
+open FStar.PCM
+open Zeta.Steel.Util
+
+let map (k:eqtype) (v:Type) = m:Map.t k v { Map.domain m `Set.equal` Set.complement Set.empty }
+let composable_maps (#a:_) (#k:eqtype)
+                    (p:pcm a)
+                    (m0 m1: map k a)
+  : prop
+  = forall k. Map.sel m0 k `composable p` Map.sel m1 k
+
+let compose_maps (#a:_) (#k:eqtype)
+                 (p:pcm a)
+                 (m0:map k a)
+                 (m1:map k a { composable_maps p m0 m1 })
+  : map k a
+  = map_literal (fun k ->
+                   Map.sel m0 k `op p` Map.sel m1 k)
+
+let composable_maps_comm #k #a
+                    (p:pcm a)
+                    (m0 m1: map k a)
+  : Lemma (composable_maps p m0 m1 <==>
+           composable_maps p m1 m0)
+  = ()
+
+
+let compose_maps_comm #k #a
+                    (p:pcm a)
+                    (m0 m1: map k a)
+  : Lemma
+    (requires composable_maps p m0 m1)
+    (ensures compose_maps p m0 m1 == compose_maps p m1 m0)
+  = let m01 = compose_maps p m0 m1 in
+    let m10 = compose_maps p m1 m0 in
+    introduce forall key.
+         Map.sel m01 key == Map.sel m10 key
+    with ( p.comm (Map.sel m0 key) (Map.sel m1 key) );
+    assert (Map.equal m01 m10)
+
+let composable_maps_assoc_l #k #a
+                          (p:pcm a)
+                          (m0 m1 m2: map k a)
+  : Lemma
+    (requires
+      composable_maps p m1 m2 /\
+      composable_maps p m0 (compose_maps p m1 m2))
+    (ensures
+      composable_maps p m0 m1 /\
+      composable_maps p (compose_maps p m0 m1) m2 /\
+      compose_maps p (compose_maps p m0 m1) m2 ==
+      compose_maps p m0 (compose_maps p m1 m2))
+  = introduce forall key.
+      composable p (Map.sel m0 key) (Map.sel m1 key)
+    with ( p.assoc (Map.sel m0 key) (Map.sel m1 key) (Map.sel m2 key) );
+    let m01 = compose_maps p m0 m1 in
+    introduce forall key.
+      composable p (Map.sel m01 key) (Map.sel m2 key)
+    with ( p.assoc (Map.sel m0 key) (Map.sel m1 key) (Map.sel m2 key) );
+    let m012 = compose_maps p m01 m2 in
+    let m012' = compose_maps p m0 (compose_maps p m1 m2) in
+    introduce forall key.
+      Map.sel m012 key == Map.sel m012' key
+    with ( p.assoc (Map.sel m0 key) (Map.sel m1 key) (Map.sel m2 key) );
+    assert (Map.equal
+                 (compose_maps p (compose_maps p m0 m1) m2)
+                 (compose_maps p m0 (compose_maps p m1 m2)))
+
+let composable_maps_assoc_r #k #a
+                          (p:pcm a)
+                          (m0 m1 m2: map k a)
+  : Lemma
+    (requires
+      composable_maps p m0 m1 /\
+      composable_maps p (compose_maps p m0 m1) m2)
+    (ensures
+      composable_maps p m1 m2 /\
+      composable_maps p m0 (compose_maps p m1 m2) /\
+      compose_maps p (compose_maps p m0 m1) m2 ==
+      compose_maps p m0 (compose_maps p m1 m2))
+  = introduce forall key.
+      composable p (Map.sel m1 key) (Map.sel m2 key)
+
+    with ( p.assoc_r (Map.sel m0 key) (Map.sel m1 key) (Map.sel m2 key) );
+    let m12 = compose_maps p m1 m2 in
+    introduce forall key.
+      composable p (Map.sel m0 key) (Map.sel m12 key)
+    with ( p.assoc_r (Map.sel m0 key) (Map.sel m1 key) (Map.sel m2 key) );
+    let m012 = compose_maps p (compose_maps p m0 m1) m2 in
+    let m012' = compose_maps p m0 (compose_maps p m1 m2) in
+    introduce forall key.
+      Map.sel m012 key == Map.sel m012' key
+    with ( p.assoc_r (Map.sel m0 key) (Map.sel m1 key) (Map.sel m2 key) );
+    assert (Map.equal m012 m012')
+
+let pcm'_map_of_pcm (#a:_) (k:eqtype) (p:pcm a)
+  : pcm' (option (map k a))
+  = {
+       composable =
+         (fun m0 m1 ->
+           match m0, m1 with
+           | None, _
+           | _, None -> True
+           | Some m0, Some m1 ->
+             composable_maps p m0 m1);
+       op = (fun m0 m1 ->
+              match m0, m1 with
+              | None, m
+              | m, None -> m
+              | Some m0, Some m1 ->
+                Some (compose_maps p m0 m1));
+       one = None;
+    }
+
+let pcm_map_of_pcm (#a:_) (k:eqtype) (p:pcm a)
+  : pcm (option (map k a))
+  = {
+       p = pcm'_map_of_pcm k p;
+       comm = (fun m0 m1 ->
+                 match m0, m1 with
+                 | None, _
+                 | _, None -> ()
+                 | Some m0, Some m1 -> compose_maps_comm p m0 m1);
+       assoc = (fun m0 m1 m2 ->
+                  match m0, m1, m2 with
+                  | Some m0, Some m1, Some m2 ->
+                    composable_maps_assoc_l p m0 m1 m2
+                  | _ -> ());
+       assoc_r = (fun m0 m1 m2 ->
+                  match m0, m1, m2 with
+                  | Some m0, Some m1, Some m2 ->
+                    composable_maps_assoc_r p m0 m1 m2
+                  | _ -> ());
+       is_unit = (fun _ -> ());
+       refine = (fun a -> Some? a /\ (forall k. p.refine (Map.sel (Some?.v a) k)))
+    }
+
+let compatible_pointwise #a #k
+                         (p:pcm a)
+                         (m0 m1:map k a)
+  : Lemma
+    (requires compatible (pcm_map_of_pcm k p) (Some m0) (Some m1))
+    (ensures forall k. compatible p (Map.sel m0 k) (Map.sel m1 k))
+  = let pcm' = pcm_map_of_pcm k p in
+    introduce forall k. compatible p (Map.sel m0 k) (Map.sel m1 k)
+    with (
+      eliminate exists frame.
+        composable pcm' (Some m0) frame /\ op pcm' frame (Some m0) == (Some m1)
+      returns _
+      with _. (
+        introduce exists (frame:a).
+                         composable p
+                                    (Map.sel m0 k)
+                                    frame /\
+                         op p frame (Map.sel m0 k) == Map.sel m1 k
+        with (match frame with None -> p.p.one | Some m -> Map.sel m k)
+        and ( p.is_unit (Map.sel m0 k);
+              p.comm p.p.one (Map.sel m0 k) ) ))
+
+
+let compatible_pointwise_upd #a (#k:eqtype)
+                             (p:pcm a)
+                             (v1 full_v1:a)
+                             (m0 full_m0:map k a)
+                             (key:k)
+  : Lemma
+    (requires
+      compatible p v1 full_v1 /\
+      compatible (pcm_map_of_pcm k p) (Some m0) (Some full_m0))
+    (ensures
+      compatible (pcm_map_of_pcm k p) (Some (Map.upd m0 key v1))
+                                      (Some (Map.upd full_m0 key full_v1)))
+  = compatible_pointwise p m0 full_m0;
+    assert (compatible p (Map.sel m0 key) (Map.sel full_m0 key));
+    let m1 = (Map.upd m0 key v1) in
+    let full_m1 = (Map.upd full_m0 key full_v1) in
+    let p' = pcm_map_of_pcm k p in
+    eliminate exists (frame_m0:_). composable p' (Some m0) frame_m0 /\ op p' frame_m0 (Some m0) == Some full_m0
+    returns _
+    with _. (
+    eliminate exists (frame0:_). composable p v1 frame0 /\ op p frame0 v1 == full_v1
+    returns _
+    with _. (
+      introduce exists (frame:_).
+      composable p' (Some m1) frame /\ op p' frame (Some m1) == (Some full_m1)
+    with (
+      match frame_m0 with
+      | None -> Some (Map.upd (Map.const p.p.one) key frame0)
+      | Some frame_m0 -> Some (Map.upd frame_m0 key frame0)
+    )
+    and (
+      match frame_m0 with
+      | None ->
+        let w = Map.upd (Map.const p.p.one) key frame0 in
+        introduce forall v.
+          composable p p.p.one v /\
+          composable p v p.p.one /\
+          op p p.p.one v == v /\
+          op p v p.p.one == v
+        with ( p.is_unit v; p.comm v p.p.one );
+        introduce forall k.
+          Map.sel m1 k `composable p` Map.sel w k
+        with (
+          if k <> key
+          then (
+            p.is_unit (Map.sel m1 k)
+          )
+        );
+        assert (composable_maps p m1 w);
+        introduce forall k.
+          Map.sel (compose_maps p w m1) k == Map.sel full_m1 k
+        with (
+            p.is_unit (Map.sel m1 k)
+        );
+        assert (Map.equal (compose_maps p w m1) full_m1)
+      | Some frame_m0 ->
+        let w = Map.upd frame_m0 key frame0 in
+        assert (Map.equal (compose_maps p w m1) full_m1)
+    )))
+
+
+let lift_fp #a (#k:eqtype) (p:pcm a)
+            (m0 full_m0:map k a)
+            (v1 full_v1:a)
+            (key:k)
+  : Lemma
+    (requires (
+      let v0 = Map.sel m0 key in
+      let full_v0 = Map.sel full_m0 key in
+      let m1 = Map.upd m0 key v1 in
+      let full_m1 = Map.upd full_m0 key full_v1 in
+      (forall (frame:a{composable p v0 frame}). {:pattern composable p v0 frame}
+         composable p v1 frame /\
+         (op p v0 frame == full_v0 ==>
+          op p v1 frame == full_v1))))
+    (ensures (
+      let v0 = Map.sel m0 key in
+      let full_v0 = Map.sel full_m0 key in
+      let m1 = Map.upd m0 key v1 in
+      let full_m1 = Map.upd full_m0 key full_v1 in
+      let p' = pcm_map_of_pcm k p in
+      (forall (frame:_{composable p' (Some m0) frame}).
+         composable p' (Some m1) frame /\
+         (op p' (Some m0) frame == (Some full_m0) ==>
+          op p' (Some m1) frame == (Some full_m1)))))
+    = let v0 = Map.sel m0 key in
+      let full_v0 = Map.sel full_m0 key in
+      let m1 = Map.upd m0 key v1 in
+      let full_m1 = Map.upd full_m0 key full_v1 in
+      let p' = pcm_map_of_pcm k p in
+      introduce forall (frame:_{composable p' (Some m0) frame}).
+         composable p' (Some m1) frame /\
+         (op p' (Some m0) frame == (Some full_m0) ==>
+          op p' (Some m1) frame == (Some full_m1))
+      with (
+        introduce _ /\ _
+        with ()
+        and ( introduce _ ==> _
+              with _. (
+                match frame with
+                | None ->
+                  assert (m0 == full_m0);
+                  p.is_unit v0;
+                  p.is_unit v1;
+                  assert (composable p v0 p.p.one);
+                  assert (v1 == full_v1);
+                  assert (m1 `Map.equal` full_m1)
+                | Some frame' ->
+                  // assert (composable p' (Some m0) (Some frame'));
+                  // assert (composable p (Map.sel m0 key) (Map.sel frame' key));
+                  // assert (Map.sel m0 key == v0);
+                  // assert (composable p v0 (Map.sel frame' key));
+                  assert (compose_maps p m1 frame' `Map.equal` full_m1)
+              )
+        )
+      )
+
+let lift_fp_upd #a #k (#p:pcm a)
+                (v0 v1:a)
+                (f:frame_preserving_upd p v0 v1)
+                (m0:map k a)
+                (key:k { Map.sel m0 key == v0 })
+  : frame_preserving_upd (pcm_map_of_pcm k p)
+                         (Some m0)
+                         (Some (Map.upd m0 key v1))
+  = fun (Some full_m0) ->
+          let p' = pcm_map_of_pcm k p in
+          let full_v0 = Map.sel full_m0 key in
+          assert (compatible (pcm_map_of_pcm _ p) (Some m0) (Some full_m0));
+          assert (p.refine full_v0);
+          compatible_pointwise #a #k p m0 full_m0;
+          assert (compatible p v0 full_v0);
+          let full_v1 = f full_v0 in
+          let full_m1 = Map.upd full_m0 key full_v1 in
+          assert (p'.refine (Some full_m1));
+          compatible_pointwise_upd p v1 full_v1 m0 full_m0 key;
+          let m1 = Map.upd m0 key v1 in
+          assert (compatible p' (Some m1) (Some full_m1));
+          lift_fp p m0 full_m0 v1 full_v1 key;
+          Some full_m1
+
+let lift_composable #k #a (p:pcm a)
+                          (v0 v1:a)
+                          (m0 m1:map k a)
+                          (key:k)
+ : Lemma (requires composable p v0 v1 /\
+                   composable (pcm_map_of_pcm k p) (Some m0) (Some m1))
+         (ensures
+                  composable (pcm_map_of_pcm k p) (Some (Map.upd m0 key v0)) (Some (Map.upd m1 key v1)))
+ = ()
